theories/Effect.v
@@ -1,0 +1,268 @@
+(* This Source Code Form is subject to the terms of the Mozilla Public
+ * License, v. 2.0. If a copy of the MPL was not distributed with this
+ * file, You can obtain one at https://mozilla.org/MPL/2.0/. *)
+
+(* Copyright (C) 2018–2020 ANSSI *)
+
+From FreerDPS Require Import Init.
+
+(** * Definition  *)
+
+(** Following the definition of the <<operational>> package, effects in
+    FreeSpec are parameterized inductive types whose terms purposely describe
+    the primitives the effect provides. *)
+
+Definition effect := Type -> Type.
+
+Declare Scope effect_scope.
+Bind Scope effect_scope with effect.
+
+(** Given [F : effect], a term of type [F α] identifies a primitive of [F]
+    expected to produce a result of type [α].
+
+    The simpler effect is the empty effect, which provides no primitives
+    whatsoever. *)
+
+Inductive eempty : effect := .
+
+(** Another example of general-purpose effect we can define is the [STORE s]
+    effect, where [s] is a type for a state, and [STORE s] allows for
+    manipulating a global, mutable variable of type [s] within an impure
+    computation. *)
+
+Inductive STORE (s : Type) : effect :=
+| Get : STORE s s
+| Put (x : s) : STORE s unit.
+
+Arguments Get {s}.
+Arguments Put [s] (x).
+
+(** According to the definition of [STORE s], an impure computation can use two
+    primitives. The term [Get : STORE s s] describes a primitive expected to
+    produce a result of type [s], that is the current value of the mutable
+    variable.  Terms of the form [Put x : STORE s unit] describe a primitive
+    which does not produce any meaningful result, but is expected to update the
+    current value of the mutable variable.
+
+    The use of the word “expected” to describe the primitive of [STORE s] is
+    voluntary.  The definition of an effect does not attach any particular
+    semantics to the primitives it describes.  This will come later, and in
+    fact, one effect may have many legitimate semantics.
+
+    Impure computations are likely to use more than one effect, but the
+    [impure] monad takes only one argument.  We introduce [eplus] (denoted by
+    [<+>] or [⊕]) to compose effects together.  An impure computation
+    parameterized by [F ⊕ E] can therefore leverage the primitives of both [F]
+    and [E]. *)
+
+(** * Polymorphic Effect Composites *)
+
+(** When defining general-purpose impure computations that we expect to reuse in
+    different context, we want to leave the effect as a parameter, and rather
+    express the constraints in terms of effect availability.  We tackle this
+    challenge by means of _effect composites_.
+
+    - We say an effect composite [Fx] _provides_ a concrete effect [F]
+      when there exists a function [inj_p : forall α, F α -> Fx α].
+    - Conversely, we can determine if a primitive of an effect composite [Fx]
+      is forwarded to a concrete effect [F] when there exists a function
+      [proj_p : forall α, Fx α -> option (F a)].
+
+    We encode this mechanics using two type classes: [MayProvide], and
+    [Provide]. *)
+
+Class MayProvide (Fx F : effect) : Type :=
+  { proj_p {α} (e : Fx α) : option (F α)
+  }.
+
+Class Provide (Fx F : effect) `{MayProvide Fx F} : Type :=
+  { inj_p {α} (e : F α) : Fx α
+  ; proj_inj_p_equ {α} (e : F α) : proj_p (inj_p e) = Some e
+  }.
+
+(** We provide a default instance for [MayProvide] in the form of a function
+    [proj_p] which always return [None].  We give to this default instance a
+    ridiculously high priority number to ensure it is selected only if no other
+    instances are found. *)
+
+Instance default_MayProvide (F E : effect) : MayProvide F E|1000 :=
+  { proj_p := fun _ _ => None
+  }.
+
+(** It is expected that, for an effect composite [Fx] which provides [F] and
+    may provide [E], [inj_p] and [proj_p] do not mix up [F] and [E]
+    primitives. That is, injecting a primitive [e] of [F] inside [Fx], then
+    projecting the resulting primitive into [E] returns [None] as long as [F]
+    and [E] are two different effects. *)
+
+Class Distinguish (Fx F E : effect) `{Provide Fx F, MayProvide Fx E} : Prop :=
+  { distinguish : forall {α} (e : F α), proj_p (F := E) (inj_p (Fx := Fx) e) = None
+  }.
+
+(** * Composing Effects *)
+
+(** We provide the [eplus] operator to compose effects together. That is,
+    [eplus] can be used to build _concrete_ (as opposed to polymorphic)
+    effect composite. *)
+
+Inductive eplus (F E : effect) (α : Type) :=
+| in_left (e : F α) : eplus F E α
+| in_right (e : E α) : eplus F E α.
+
+Arguments in_left [F E α] (e).
+Arguments in_right [F E α] (e).
+
+Register eplus as freespec.core.eplus.type.
+Register in_left as freespec.core.eplus.in_left.
+Register in_right as freespec.core.eplus.in_right.
+
+Infix "+" := eplus : effect_scope.
+
+(** For [eplus] to be used seamlessly as a concrete effect composite, we
+    provide the necessary instances for the [MayProvide], [Provide] and
+    [Distinguish] type classes. Note that these instances always prefer the
+    left operand of [eplus]. For instance, considering a situation where
+    there is an instance for [Provide Fx F] and an instance for [Provide Ex F],
+    the instance of [Provide (Fx + Ex) F] will rely on [Fx].
+
+    The main use case for [eplus] is to locally provide an additional
+    effect. For instance, we can consider a [with_state] function which would
+    locally give access to the [STORE] effect, that is [with_state : forall
+    Fx s α, s -> impure (Fx + STORE s) α -> impure Fx α]. In such a case, the
+    effect made locally available shall be the right operand of [eplus]. This
+    way, functions such as [with_state] are reentrant. If we take an example,
+    the following impure computation:
+
+<<
+with_state true (with_state false get)
+>>
+
+    will return false (that is, the variable in the inner store). *)
+
+Instance refl_MayProvide (F : effect) : MayProvide F F :=
+  { proj_p := fun _ e => Some e
+  }.
+
+#[program]
+Instance refl_Provide (F : effect) : @Provide F F (refl_MayProvide F) :=
+  { inj_p := fun (a : Type) (e : F a) => e
+  }.
+
+Instance eplus_left_MayProvide (Fx F E : effect) `{MayProvide Fx F}
+  : MayProvide (Fx + E) F :=
+  { proj_p := fun _ e =>
+                match e with
+                | in_left e => proj_p e
+                | _ => None
+                end
+  }.
+
+#[program]
+Instance eplus_left_Provide (Fx F E : effect) `{Provide Fx F}
+  : @Provide (Fx + E) F (eplus_left_MayProvide Fx F E) :=
+  { inj_p := fun (a : Type) (e : F a) => in_left (inj_p e)
+  }.
+
+Next Obligation.
+  now rewrite proj_inj_p_equ.
+Qed.
+
+Instance eplus_right_MayProvide (F Ex E : effect) `{MayProvide Ex E}
+  : MayProvide (F + Ex) E :=
+  { proj_p := fun _ e =>
+                match e with
+                | in_right e => proj_p e
+                | _ => None
+                end
+  }.
+
+#[program]
+Instance eplus_right_Provide (F Ex E : effect) `{Provide Ex E}
+  : @Provide (F + Ex) E (eplus_right_MayProvide F Ex E) :=
+  { inj_p := fun _ e => in_right (inj_p e)
+  }.
+
+Next Obligation.
+  now rewrite proj_inj_p_equ.
+Qed.
+
+(** By default, Coq's inference algorithm for type classe instances inference is
+    a depth-first search. This is not without consequence in our case. For
+    instance, if we consider the search of an instance for [MayProvide (F + E)
+    E], Coq will first try [eplus_right_MayProvide] (as explained previously),
+    meaning he now search for [MayProvide F E]. It turns out such an instance
+    exists: [default_MayProvide].
+
+    To circumvent this issue, we write a dedicated tactic [find_may_provide]
+    which attempts to find an instance for [MayProvide (?Fx + ?Ex) ?F] with
+    [refl_MayProvide], [eplus_left_MayProvide] and [eplus_right_MayProvide]. *)
+
+Ltac find_may_provide :=
+  eapply refl_MayProvide +
+  (eapply eplus_left_MayProvide; find_may_provide) +
+  (eapply eplus_right_MayProvide; find_may_provide).
+
+#[global] Hint Extern 1 (MayProvide (eplus _ _) _) =>
+  find_may_provide : typeclass_instances.
+
+#[program]
+Instance refl_Distinguish (F E : effect)
+  : @Distinguish F F E  ( @refl_MayProvide F) ( @refl_Provide F) ( @default_MayProvide F E).
+
+#[program]
+Instance eplus_left_default_Distinguish (Fx Ex F E : effect)
+   `{M1 : MayProvide Fx F} `{P1 : @Provide Fx F M1}
+  : @Distinguish (Fx + Ex) F E
+                 ( @eplus_left_MayProvide Fx F Ex M1)
+                 ( @eplus_left_Provide Fx F Ex M1 P1)
+                 ( @default_MayProvide _ E).
+
+#[program]
+Instance eplus_right_default_Distinguish (Fx Ex F E : effect)
+   `{M1 : MayProvide Ex F} `{P1 : @Provide Ex F M1}
+  : @Distinguish (Fx + Ex) F E
+                 ( @eplus_right_MayProvide Fx Ex F M1)
+                 ( @eplus_right_Provide Fx Ex F M1 P1)
+                 ( @default_MayProvide _ E).
+
+#[program]
+Instance eplus_left_may_right_Distinguish (Fx Ex F E : effect)
+   `{M1 : MayProvide Fx F} `{P1 : @Provide Fx F M1} `{M2 : MayProvide Ex E}
+  : @Distinguish (Fx + Ex) F E
+                 ( @eplus_left_MayProvide Fx F Ex M1)
+                 ( @eplus_left_Provide Fx F Ex M1 P1)
+                 ( @eplus_right_MayProvide Fx Ex E M2).
+
+#[program]
+Instance eplus_right_may_left_Distinguish (Fx Ex F E : effect)
+   `{M1 : MayProvide Ex F} `{P1 : @Provide Ex F M1} `{M2 : MayProvide Fx E}
+  : @Distinguish (Fx + Ex) F E
+                 ( @eplus_right_MayProvide Fx Ex F M1)
+                 ( @eplus_right_Provide Fx Ex F M1 P1)
+                 ( @eplus_left_MayProvide Fx E Ex M2).
+
+#[program]
+Instance eplus_left_distinguish_left_Distinguish (Fx Ex F E : effect)
+   `{M1 : MayProvide Fx F} `{P1 : @Provide Fx F M1} `{M2 : MayProvide Fx E}
+   `{@Distinguish Fx F E M1 P1 M2}
+  : @Distinguish (Fx + Ex) F E
+                 ( @eplus_left_MayProvide Fx F Ex M1)
+                 ( @eplus_left_Provide Fx F Ex M1 P1)
+                 ( @eplus_left_MayProvide Fx E Ex M2).
+
+Next Obligation.
+  apply distinguish.
+Defined.
+
+#[program]
+Instance eplus_right_distinguish_right_Distinguish (Fx Ex F E : effect)
+   `{M1 : MayProvide Ex F} `{P1 : @Provide Ex F M1} `{M2 : MayProvide Ex E}
+   `{@Distinguish Ex F E M1 P1 M2}
+  : @Distinguish (Fx + Ex) F E
+                 ( @eplus_right_MayProvide Fx Ex F M1)
+                 ( @eplus_right_Provide Fx Ex F M1 P1)
+                 ( @eplus_right_MayProvide Fx Ex E M2).
+
+Next Obligation.
+  apply distinguish.
+Defined.
